\subsection{Inverse Operator($E^{-1}$)}

\begin{enumerate}
  \item The inverse operator is defined as the difference between the function values at two consecutive points.
  \item The inverse operator is denoted by $E^{-1}$.

  \mybox{
    General Relation : \\
  
    \[{E}^{-m} y_n = {y}_{n - m}\]

}

  \[E^{-1} f(a - h) = f(a) \]
  \[E^{-1} f(a + 2h) = f(a + h) \]
  \[E^{-1} f(a + 3h) = f(a + 2h) \]
  \[E^{-1} f(a + 4h) = f(a + 3h) \]
  \[E^{-1} f(a + 5h) = f(a + 4h) \]

  \mybox{
    Example :
    \[E^{-1} sin(x) = sin(x-h) \]
    \[E^{-1} e^{2(x+h)} = e^{2(x-h)}\]
  }

  
\end{enumerate}

\subsubsection{$n^{th}$ Inverse Operator($E^{-n}$)}

\[E^{-n} f(a + nh) = f(a)\]

\mybox{
    Example :
    \[E^{-2} f(a + h) = f(a - h)\]
    \[E^{-3} f(a + 3h) = f(a)\]
    \[E^{-4} f(a) = f(a -4h)\]
}

\subsubsection{Some Examples of Inverse Operator($E^{-1}$)}

\[E^{-1} y_0 = {y}_{-1}\]
\[E^{-1} y_1 = y_0\]
\[E^{-1} y_5 = y_4\]
\[E^{-2} y_0 = {y}_{-2}\]
\[E^{-2} y_3 = y_1\]
\[E^{-3} y_6 = {y}_{-3}\]